work in progress

bedrock2/src/bedrock2Examples/roughtime.v
@@ -1,10 +1,29 @@
+Ltac pick_nat n :=
+  multimatch n with
+  | S ?m => constr:(m)
+  | S ?m => pick_nat m
+  end.
+
+
+Require Import bedrock2.Array bedrock2.Scalars.
+From bedrock2.Map Require Import Separation SeparationLogic.
+
+(*Changed array_append' to array_append*)
+Ltac get_array_rewr_eq t :=
+  lazymatch t with
+  | context [ array ?PT ?SZ ?start (?xs ++ ?ys) ] =>
+    constr:(iff1ToEq (array_append PT SZ xs ys start))
+  | context [ array ?PT ?SZ ?start (?x :: ?xs) ] =>
+    constr:(iff1ToEq (array_cons PT SZ x xs start))
+  | context [ array ?PT ?SZ ?start nil ] =>
+    constr:(iff1ToEq (array_nil PT SZ start))
+  end.
+
 
 Require Import bedrock2.Syntax bedrock2.NotationsInConstr bedrock2.NotationsCustomEntry.
-Require Import bedrock2.Array bedrock2.Scalars.
 Import Syntax BinInt String List.ListNotations ZArith.
 From coqutil Require Import Word.Interface Map.Interface.
-Require Import coqutil.Byte coqutil.Z.HexNotation.
-From bedrock2.Map Require Import Separation SeparationLogic.
+Require Import coqutil.Byte coqutil.Z.HexNotation coqutil.Z.Lia.
 
 Local Open Scope string_scope. Local Open Scope Z_scope. Local Open Scope list_scope.
 Local Coercion literal (z : Z) : Syntax.expr := Syntax.expr.literal z.
@@ -13,14 +32,14 @@ Local Definition bedrock_func : Type :=
   String.string * (list String.string * list String.string * cmd).
 Local Coercion name_of_func (f : bedrock_func) := fst f.
 
-Definition stringToHex (s : string) : Z.
-Admitted.
+Definition stringToHex (s : string) : Z := Ox"ffffffff".
 
 Lemma stringHexBound : forall s, 0 <= stringToHex s < 2^32.
-Proof. Admitted.
+Proof. intros s. unfold stringToHex. cbn. blia. Qed.
 
 Definition createTimestampMessage :=
   let buffer := "buffer" in
+  let i := "i" in
   ("createTimestampMessage", ([buffer], []:list String.string, bedrock_func_body:(
     store4(buffer, constr:(Ox"5"));
     store4(buffer + constr:(4), constr:(Ox"40"));
@@ -32,8 +51,22 @@ Definition createTimestampMessage :=
     store4(buffer + constr:(24), constr:(stringToHex "PATH"));
     store4(buffer + constr:(28), constr:(stringToHex "SREP"));
     store4(buffer + constr:(32), constr:(stringToHex "CERT"));
-    store4(buffer + constr:(36), constr:(stringToHex "INDX"))
+    store4(buffer + constr:(36), constr:(stringToHex "INDX"));
 
+    i = (constr:(64)); while (i) { i = (i - constr:(4));
+      store4(buffer + constr:(100) - i, constr:(Ox"42"))
+    };
+
+    store4(buffer + constr:(104), constr:(Ox"3"));
+    store4(buffer + constr:(108), constr:(Ox"4"));
+    store4(buffer + constr:(112), constr:(Ox"c"));
+
+    store4(buffer + constr:(116), constr:(stringToHex "RADI"));
+    store4(buffer + constr:(120), constr:(stringToHex "MIDP"));
+    store4(buffer + constr:(124), constr:(stringToHex "ROOT"));
+    
+    store4(buffer + constr:(128), constr:(Ox"42424242"));
+    store(buffer + constr:(232), constr:(Ox"4242424242424242"))
   ))).
 
 Require bedrock2.WeakestPrecondition.
@@ -44,46 +77,86 @@ Require Import bedrock2.Map.Separation bedrock2.Map.SeparationLogic.
 Require bedrock2.WeakestPreconditionProperties.
 From coqutil.Tactics Require Import letexists eabstract.
 Require Import bedrock2.ProgramLogic bedrock2.Scalars.
-Require Import coqutil.Z.Lia coqutil.Word.Properties.
+Require Import coqutil.Z.Lia coqutil.Word.Properties bedrock2.TailRecursion.
+
+(* This can be overridden by the user.
+   The idea of a "tag" is that it's a subterm of a sepclause which is so unique that if
+   the same tag appears both on the left and on the right of an iff1, we're sure that
+   these two clauses should be matched & canceled with each other.
+   "tag" should return any Gallina term. *)
+Ltac tag P :=
+  let __ := lazymatch type of P with
+            | @map.rep _ _ _ -> Prop => idtac
+            | _ => fail 10000 P "is not a sep clause"
+            end in
+  lazymatch P with
+  | _ => fail "no recognizable tag"
+  end.
+
+(* This can be overridden by the user.
+   The idea of "addr" is that if the addresses of two sepclauses are the same,
+   we're sure that these two clauses should be matched & canceled with each other,
+   even if they still contain many evars outside of their address.
+   "addr" should return a Gallina term of type "word" *)
+Ltac addr P :=
+  let __ := lazymatch type of P with
+            | @map.rep _ _ _ -> Prop => idtac
+            | _ => fail 10000 P "is not a sep clause"
+            end in
+  lazymatch P with
+  | ptsto ?A _ => A
+  | ptsto_word ?A _ => A
+  | array _ _ ?A _ => A
+  | _ => fail "no recognizable address"
+  end.
 
 
+Import coqutil.Tactics.rdelta.
+Require Import coqutil.Tactics.rewr.
 
+Ltac array_app_cons_sep := rewr get_array_rewr_eq in *.
+
+Ltac wseplog_pre :=
+  repeat (autounfold with unf_to_array);
+  repeat ( rewr get_array_rewr_eq in |-* ).
 
 Section WithParameters.
   Context {p : FE310CSemantics.parameters}.
 
   Definition entry: Type := string * Semantics.word * (Semantics.word -> mem -> Prop).
 
-  Local Infix "*" := (sep).
-  Local Infix "*" := (sep) : type_scope.
+  Infix "*" := (sep).
+  Infix "*" := (sep) : type_scope.
+
   Local Infix "+" := word.add.
   Notation array32 := (array scalar32 (word.of_Z 4)).
+  
   Definition stringToWord (s : string) := word.of_Z (stringToHex s).
 
-
-  Definition size_ok (addr: Semantics.word) (entries : list entry) : mem -> Prop :=
+  Definition size_field (addr: Semantics.word) (entries : list entry) : mem -> Prop :=
     scalar32 addr (word.of_Z (Z.of_nat (List.length entries))).
-  Definition offsets_ok (addr: Semantics.word) (entries : list entry) : mem -> Prop :=
-    array32 (addr + (word.of_Z 4)) (match entries with | [] => [] | h::tail =>
-            (List.map (fun entry => stringToWord (fst (fst entry))) tail) end).
-  Definition tags_offset (sz: nat) := match sz with
-                                    | (0%nat) => 4%nat
-                                    | _ => (4%nat * sz)%nat
-                                    end.
-  Definition tags_ok (addr: Semantics.word) (entries : list entry) : mem -> Prop :=
-    array32 (addr + (word.of_Z (Z.of_nat (tags_offset (List.length entries)))))
+  
+  Definition offsets_field (addr: Semantics.word) (entries : list entry) : mem -> Prop :=
+    array32 (addr + (word.of_Z 4)) 
+            (List.map (fun entry => (snd (fst entry))) (tl entries)).
+  
+  Definition tags_offset (entries : list entry) :=
+    (4 + 4 * (List.length (tl entries)))%nat.
+  
+  Definition tags_field (addr: Semantics.word) (entries : list entry) : mem -> Prop :=
+    array32 (addr + (word.of_Z (Z.of_nat (tags_offset entries))))
             (List.map (fun entry => stringToWord (fst (fst entry))) entries).
 
-  Definition contents_offset (sz: nat) := (tags_offset sz + sz)%nat.
+  Definition contents_offset (entries : list entry) :=
+    (tags_offset entries + 4 * (List.length entries))%nat.
   
-  Fixpoint message_ok (addr: Semantics.word) (entries : list entry): mem -> Prop :=
-    size_ok addr entries * offsets_ok addr entries * tags_ok addr entries *
-    let current_addr := addr + (word.of_Z (Z.of_nat (contents_offset (List.length entries)))) in
+  Definition message_ok (addr: Semantics.word) (entries : list entry): mem -> Prop :=
+    size_field addr entries * offsets_field addr entries * tags_field addr entries *
+    let current_addr := addr + (word.of_Z (Z.of_nat (contents_offset entries))) in
     List.fold_left (fun P entry => (snd entry) (current_addr + (snd (fst entry))) * P)
                    entries (emp True).
-
   
-  Definition repeat_dummy n := fun addr => array32 addr (List.repeat (word.of_Z 66) n).
+  Definition repeat_dummy n := fun addr => array32 (addr: Semantics.word) (List.repeat (word.of_Z 66) n).
 
   Definition srep_val : list entry :=
     [("RADI", word.of_Z 0, repeat_dummy 4);
@@ -103,7 +176,7 @@ Section WithParameters.
   Instance spec_of_createTimestampMessage : spec_of "createTimestampMessage" := fun functions =>
     forall p_addr buf R m t,
       ((array32 p_addr buf) * R) m ->
-      List.length buf = 10%nat ->
+      List.length buf = 1024%nat ->
       WeakestPrecondition.call functions "createTimestampMessage" t m [p_addr]
       (fun t' m' rets => t = t' /\ rets = nil /\ (message_ok p_addr message_val * R) m'). 
   
@@ -111,14 +184,760 @@ Section WithParameters.
         (preprocess [autorewrite with rew_word_morphism],
          morphism (Properties.word.ring_morph (word := Semantics.word)),
          constants [Properties.word_cst]).
-
+(*
    Lemma word_add_simplify (w: Semantics.word) (x y: Z) :
         w + (word.of_Z x) + (word.of_Z y) = w + (word.of_Z (x + y)).
    Proof.
      ring.
    Qed.
+*)
+   Require Import coqutil.Tactics.Tactics.
+   (*
+   Ltac word_simplify :=
+     repeat (rewrite word_add_simplify in * ); cbv[Z.add Pos.add Pos.succ] in *.
+*)
+   Ltac foo := idtac.
+   
+   Ltac canonicalize_word_width_and_instance :=  repeat so fun hypergoal => 
+     match hypergoal with
+     | context [@word.unsigned ?wi ?inst] =>
+       let wi' := eval cbn in wi in let inst' := eval cbn in inst in
+          progress (change wi with wi' in *; change inst with inst' in * ) 
+     | context [@word.signed   ?wi ?inst] => let wi' := eval cbn in wi in let inst' := eval cbn in inst in
+          progress ( change wi with wi' in *; change inst with inst' in * ) 
+     end.
 
-   Ltac word_simplify := repeat (rewrite word_add_simplify in *); cbv[Z.add Pos.add Pos.succ] in *.
+  
+   Ltac subst_words :=
+     repeat match goal with x := _ : word.rep |- _ => subst x end.
+   
+   Notation "a |-> v" := (scalar32 a (word.of_Z v)) (at level 30).
+   Notation lit := (@word.of_Z (@width (@semantics_parameters p))
+            (@Semantics.word (@semantics_parameters p))).
+
+   Ltac word_simplify :=
+       match goal with
+       | |- context [?a + ?b] => progress (ring_simplify (a + b))
+       | |- context [word.sub ?a ?b] => progress (ring_simplify (word.sub a b))
+       | |- context [ (word.unsigned (word.of_Z ?z))] => rewrite (word.unsigned_of_Z z); replace (word.wrap z) with z by (cbn; blia)
+       | |- context [word.of_Z (word.unsigned ?z)] => rewrite (word.of_Z_unsigned z)
+       | H: context [?a + ?b] |- _ => progress (ring_simplify (a + b) in H)
+       | H: context [word.sub ?a ?b] |- _ => progress (ring_simplify (word.sub a b) in H)
+       | H: context [word.unsigned (word.of_Z ?z)] |- _ => rewrite (word.unsigned_of_Z z) in H; replace (word.wrap z) with z in H by (cbn; blia)
+       | H: context [word.of_Z (word.unsigned ?z)] |- _ => rewrite (word.of_Z_unsigned z) in H
+       end.
+
+
+   Ltac word_unsigned z := rewrite (word.unsigned_of_Z z); replace (word.wrap z) with z by (cbn; blia).
+     
+   
+   Lemma createTimestampMessage_ok : program_logic_goal_for_function! createTimestampMessage.
+   Proof.
+     repeat straightline.
+     do 10 (destruct buf; [inversion H0|]).
+     inversion H0; clear H0.
+     cbn[Array.array] in H.
+
+     repeat word_simplify.
+     repeat straightline.
+     subst_words.
+     clear H9 H8 H7 H6 H5 H4 H3 H1 H0 H.
+     repeat word_simplify.
+     
+     refine ((TailRecursion.atleastonce ["i"; "buffer"] (fun V T M I BUFFER =>
+       exists i, V = 64 - 4 * (Z.of_nat i) /\
+       V = word.unsigned I /\ V <> 0 /\ BUFFER = p_addr /\ (array32 (p_addr + (lit 40)) (List.repeat (word.of_Z (Ox"42")) i) * array32 (p_addr + (lit (104 - V))) (List.skipn i buf) *
+         (p_addr + lit 36) |-> 4294967295 *
+         (word.add p_addr (lit 32) |-> 4294967295 *
+          (word.add p_addr (lit 28) |-> 4294967295 *
+           (word.add p_addr (lit 24) |-> 4294967295 *
+            (word.add p_addr (lit 20) |-> 4294967295 *
+             (word.add p_addr (lit 16) |-> 316 *
+              (word.add p_addr (lit 12) |-> 164 *
+               (word.add p_addr (lit 8) |-> 64 *
+                (word.add p_addr (lit 4) |-> 64 *
+                 (p_addr |-> 5 * R)))))))))%type) M
+       )) _ _ _ _ _ _ _);
+      cbn [reconstruct map.putmany_of_list HList.tuple.to_list
+           HList.hlist.foralls HList.tuple.foralls
+           HList.hlist.existss HList.tuple.existss
+           HList.hlist.apply  HList.tuple.apply
+           HList.hlist
+
+           List.repeat Datatypes.length
+           HList.polymorphic_list.repeat HList.polymorphic_list.length
+           PrimitivePair.pair._1 PrimitivePair.pair._2] in *.
+     
+     { repeat straightline. }
+     { eapply (Z.lt_wf 0). }
+     { repeat straightline.
+       shelve. }
+     { exists 0%nat.
+       repeat (split; trivial; []).
+       repeat word_simplify.
+       split; try split; try split; try blia; auto.
+       cbn [List.repeat Array.array List.skipn].
+       ecancel_assumption. }
+                             idtac.
+     do 10 straightline.
+     do 10 straightline.
+     do 2 straightline.
+     straightline_cleanup.
+     subst_words.
+     repeat word_simplify.
+     
+     assert (x = lit v).
+     { subst v; rewrite word.of_Z_unsigned; auto. }
+     rewrite H.
+     assert (List.length (List.skipn (Z.to_nat ((64 - v) / 4)) buf) <> 0%nat).
+     { rewrite List.skipn_length, H2. admit. }
+     destruct (List.skipn (Z.to_nat ((64 - v) / 4)) buf) eqn:H17; try contradiction.
+     array_app_cons_sep.
+     word_simplify.
+     repeat straightline.
+     { subst_words.
+       subst v.
+       rewrite word.of_Z_unsigned in *.
+       eexists; auto.
+       split.
+       - split; auto.
+         split; try split; try split; auto; try blia.
+         { rewrite word.unsigned_sub.
+           word_simplify.
+           admit. }
+         use_sep_assumption.
+         cancel.
+         cancel_seps_at_indices 2%nat 1%nat.
+         { repeat word_simplify.
+           f_equal.
+           admit. }
+         repeat word_simplify.
+         replace (Z.to_nat ((64 - word.unsigned (word.sub x0 (lit 4))) / 4)) with ((Z.to_nat ((64 - word.unsigned x0) / 4)) + 1)%nat by admit.
+
+     
+
+     refine ((TailRecursion.atleastonce ["i"; "buffer"] (fun V T M I BUFFER =>
+       let i := Z.to_nat ((64 - V) / 4) in
+       V = word.unsigned I /\ V <> 0 /\ V <= 64 /\ BUFFER = p_addr /\ (array32 (p_addr + (lit 40)) (List.repeat (word.of_Z (Ox"42")) i) * array32 (p_addr + (lit (104 - V))) (List.skipn i buf) *
+         (p_addr + lit 36) |-> 4294967295 *
+         (word.add p_addr (lit 32) |-> 4294967295 *
+          (word.add p_addr (lit 28) |-> 4294967295 *
+           (word.add p_addr (lit 24) |-> 4294967295 *
+            (word.add p_addr (lit 20) |-> 4294967295 *
+             (word.add p_addr (lit 16) |-> 316 *
+              (word.add p_addr (lit 12) |-> 164 *
+               (word.add p_addr (lit 8) |-> 64 *
+                (word.add p_addr (lit 4) |-> 64 *
+                 (p_addr |-> 5 * R)))))))))%type) M
+       )) _ _ _ _ _ _ _);
+      cbn [reconstruct map.putmany_of_list HList.tuple.to_list
+           HList.hlist.foralls HList.tuple.foralls
+           HList.hlist.existss HList.tuple.existss
+           HList.hlist.apply  HList.tuple.apply
+           HList.hlist
+
+           List.repeat Datatypes.length
+           HList.polymorphic_list.repeat HList.polymorphic_list.length
+           PrimitivePair.pair._1 PrimitivePair.pair._2] in *.
+     { repeat straightline. }
+     { eapply (Z.lt_wf 0). }
+     { repeat straightline.
+       shelve. }
+     { repeat (split; trivial; []).
+       repeat word_simplify.
+       split; try split; try split; try blia; auto.
+       simpl (Z.to_nat _).
+       cbn [List.repeat Array.array List.skipn].
+       ecancel_assumption. }
+     
+     
+     repeat straightline.
+     subst_words.
+     repeat word_simplify.
+     assert (x = lit v).
+     { subst v; rewrite word.of_Z_unsigned; auto. }
+     rewrite H.
+     assert (List.length (List.skipn (Z.to_nat ((64 - v) / 4)) buf) <> 0%nat).
+     { rewrite List.skipn_length, H2. admit. }
+     destruct (List.skipn (Z.to_nat ((64 - v) / 4)) buf) eqn:H17; try contradiction.
+     array_app_cons_sep.
+     word_simplify.
+     repeat straightline.
+     { subst_words.
+       subst v.
+       rewrite word.of_Z_unsigned in *.
+       eexists; auto.
+       split.
+       - split; auto.
+         split; try split; try split; auto; try blia.
+         { rewrite word.unsigned_sub.
+           word_simplify.
+           admit. }
+         use_sep_assumption.
+         cancel.
+         cancel_seps_at_indices 2%nat 1%nat.
+         { repeat word_simplify.
+           f_equal.
+           admit. }
+         repeat word_simplify.
+         replace (Z.to_nat ((64 - word.unsigned (word.sub x0 (lit 4))) / 4)) with ((Z.to_nat ((64 - word.unsigned x0) / 4)) + 1)%nat by admit.
+         match goal with
+         | |- context [List.repeat ?x (?n + 1)] =>
+           replace (List.repeat x (n + 1)) with (List.repeat x n ++ [x]); idtac n
+         end.
+         { array_app_cons_sep.
+           rewrite List.repeat_length.
+           rewrite word.unsigned_of_Z.
+           change (word.wrap 4) with 4.
+           rewrite ZifyInst.of_nat_to_nat_eq.
+           assert (0 <> ((64 - word.unsigned x0) / 4)).
+           Search 
+           { blia.
+           unfold Z.max.
+           Search Z.of_nat Z.to_nat.
+           Search word.of_Z.
+           word_simplify.
+           rewrite word.of_Z_unsigned.
+           repeat word_simplify.
+           
+           
+           match goal with
+           | |- context [ @array ?w ?word ?v ?m ?T ?PT ?SZ ?start (?xs ++ ?ys) ] =>
+             pose proof iff1ToEq (@array_append w word _ v m _ T PT SZ xs ys start); idtac T
+           end.
+           rewrite H.
+           Set Printing All.
+           pose proof iff1ToEq (array_append scalar32 (word.of_Z 4) (List.repeat (lit (Ox "42")) x1) [lit (Ox "42")] (word.add p_addr (lit 40))).
+           Unset Printing All.
+           rewrite H21.
+           Set Printing All.
+           
+           word_simplify.
+         exists (x1 + 1)%nat.
+         split. 1: admit.
+         split. 1: admit.
+         use_sep_assumption.
+         cancel.
+         cancel_seps_at_indices 2%nat 1%nat.
+         { destruct buf; try inversion H2.
+           replace (x1 + 1)%nat with (S x1) by blia.
+           rewrite List.skipn_cons.
+           admit. }
+       
+       simpl.
+       exists 0%nat; split; try blia.
+       split; try f_equal.
+       cbn [List.repeat Array.array List.skipn].
+       repeat word_simplify.
+       ecancel_assumption. }
+     repeat straightline.
+     subst_words.
+     replace (word.sub (p_addr + lit 104) (word.sub (lit (Z.of_nat (64 - 4 * x1))) (lit 4))) with (word.add (word.add p_addr (word.of_Z 40)) (word.of_Z (Z.of_nat (4 * x1)))) by admit.
+     
+     
+
+     
+     
+
+     refine ((TailRecursion.atleastonce ["i"; "buffer"] (fun V T M I BUFFER =>
+       V = word.unsigned I /\ word.unsigned I <> 0 /\ BUFFER = p_addr /\ exists i, (i < 16)%nat /\ I = word.of_Z (Z.of_nat (64 - 4*i)%nat) /\ (array32 (word.add BUFFER (word.of_Z 40)) (List.repeat (lit (Ox"42")) i) * array32 (word.add (word.add p_addr (word.of_Z 40)) (word.of_Z (Z.of_nat (4*i)%nat))) (List.skipn i buf) *
+         (p_addr + lit 36) |-> lit 4294967295 *
+         (word.add p_addr (lit 32) |-> lit 4294967295 *
+          (word.add p_addr (lit 28) |-> lit 4294967295 *
+           (word.add p_addr (lit 24) |-> lit 4294967295 *
+            (word.add p_addr (lit 20) |-> lit 4294967295 *
+             (word.add p_addr (lit 16) |-> lit 316 *
+              (word.add p_addr (lit 12) |-> lit 164 *
+               (word.add p_addr (lit 8) |-> lit 64 *
+                (word.add p_addr (lit 4) |-> lit 64 *
+                 (p_addr |-> lit 5 * R)))))))))%type) M
+       )) _ _ _ _ _ _ _);
+      cbn [reconstruct map.putmany_of_list HList.tuple.to_list
+           HList.hlist.foralls HList.tuple.foralls
+           HList.hlist.existss HList.tuple.existss
+           HList.hlist.apply  HList.tuple.apply
+           HList.hlist
+
+           List.repeat Datatypes.length
+           HList.polymorphic_list.repeat HList.polymorphic_list.length
+           PrimitivePair.pair._1 PrimitivePair.pair._2] in *.
+
+     { repeat straightline. }
+     { eapply (Z.lt_wf 0). }
+     { repeat straightline.
+       shelve. }
+     { repeat (split; trivial; []).
+       split; try split; auto.
+       { rewrite word.unsigned_of_Z; cbn; blia. }
+       exists 0%nat; split; try blia.
+       split; try f_equal.
+       cbn [List.repeat Array.array List.skipn].
+       repeat word_simplify.
+       ecancel_assumption. }
+     repeat straightline.
+     subst_words.
+     replace (word.sub (p_addr + lit 104) (word.sub (lit (Z.of_nat (64 - 4 * x1))) (lit 4))) with (word.add (word.add p_addr (word.of_Z 40)) (word.of_Z (Z.of_nat (4 * x1)))) by admit.
+     assert (List.length (List.skipn x1 buf) <> 0%nat).
+     { rewrite List.skipn_length; blia. }
+     destruct (List.skipn x1 buf) eqn:H17; try contradiction.
+     array_app_cons_sep.
+     repeat straightline.
+     { eexists; auto.
+       subst_words.
+       split.
+       - split; auto.
+         split; try split; auto; try blia.
+         exists (x1 + 1)%nat.
+         split. 1: admit.
+         split. 1: admit.
+         use_sep_assumption.
+         cancel.
+         cancel_seps_at_indices 2%nat 1%nat.
+         { destruct buf; try inversion H2.
+           replace (x1 + 1)%nat with (S x1) by blia.
+           rewrite List.skipn_cons.
+           admit. }
+         Set Printing All.
+         match goal with
+         | |- context [List.repeat ?x (?n + 1)] =>
+           replace (List.repeat x (n + 1)) with (List.repeat x n ++ [x])
+         end.
+         Set Printing All.
+         {
+           match goal with
+           | |- context [ @array ?w ?word ?v ?m ?T ?PT ?SZ ?start (?xs ++ ?ys) ] =>
+             pose proof iff1ToEq (@array_append w word _ v m _ T PT SZ xs ys start)
+           end.
+           Set Printing All.
+           rewrite H13.
+           array_app_cons_sep.
+         
+     destruct (List.skipn x1 bufl) eqn:H20; try contradiction.
+     cbn[Array.array] in H19.
+     repeat straightline.
+     { eexists; auto.
+       subst v9 x.
+       split.
+       - split; auto.
+         split; try split; auto; try blia.
+         exists (x1 + 1)%nat.
+         split. 1: admit.
+         split. 1: admit.
+         use_sep_assumption.
+         cancel.
+         cancel_seps_at_indices 2%nat 1%nat.
+
+     
+     word_simplify.
+     (word.sub (p_addr + lit 104) (word.sub (lit (Z.of_nat (64 - 4 * x1))) (lit 4)))
+    
+     Search Z.of_nat.
+     
+       simpl (Z.of_nat (4 * 0)).
+       cbn [Z.of_nat (4 * 0)].
+       
+       
+       
+       subst i; split; try split; auto.
+       - rewrite word.unsigned_of_Z.
+         unfold word.wrap.
+         change width with 32.
+         admit.
+       - exists 0%nat; split; try blia.
+         split; try f_equal.
+         cbn [List.repeat Array.array].
+         replace (word.add (word.add p_addr (word.of_Z 40)) (word.of_Z (Z.of_nat (4 * 0)))) with (word.add p_addr (word.of_Z 40)) by admit.
+         rewrite List.skipn_O.
+         ecancel_assumption. }
+     repeat straightline.
+     subst i a8 x.
+     replace (word.sub (p_addr + word.of_Z 104)
+       (word.sub (word.of_Z (Z.of_nat (64 - 4 * x1))) (word.of_Z 4))) with (word.add (word.add p_addr (word.of_Z 40)) (word.of_Z (Z.of_nat (4 * x1)))) by admit.
+
+     assert (List.length (List.skipn x1 bufl) <> 0%nat).
+     { rewrite List.skipn_length.
+       rewrite H11.
+       blia. }
+     
+     
+          
+     rewrite <- (List.firstn_skipn 16 buf) in H10.
+     set (bufr := List.skipn 16 buf) in *.
+     set (bufl := List.firstn 16 buf) in *.
+     assert (List.length bufl = 16%nat).
+     { subst bufl. rewrite List.firstn_length_le; blia. }
+     assert (List.length bufr = 998%nat).
+     { subst bufr. rewrite List.skipn_length; blia. }
+
+     
+     array_app_cons_sep.
+     rewrite H11 in H10.
+     repeat word_simplify.
+
+     
+
+     (*
+     pose proof (array_append scalar32 (word.of_Z 4) bufl bufr) (p_addr + (word.of_Z 40)).
+     rewrite H11 in H13.
+     replace (word.add (word.add p_addr (word.of_Z 40))
+                       (word.of_Z (word.unsigned (word.of_Z 4) * Z.of_nat 16))) with
+         (word.add p_addr (word.of_Z 104)) in H13.
+     2: { rewrite word.unsigned_of_Z. simpl. rewrite word_add_simplify.
+          reflexivity. }
+     
+     SeparationLogic.seprewrite_in H13 H10.
+     *)
+     refine ((TailRecursion.atleastonce ["i"; "buffer"] (fun V T M I BUFFER =>
+       V = word.unsigned I /\ word.unsigned I <> 0 /\ BUFFER = p_addr /\ exists i, (i < 16)%nat /\ I = word.of_Z (Z.of_nat (64 - 4*i)%nat) /\ (array32 (word.add BUFFER (word.of_Z 40)) (List.repeat (lit (Ox"42")) i) * (array32 (word.add (word.add p_addr (word.of_Z 40)) (word.of_Z (Z.of_nat (4*i)%nat))) (List.skipn i bufl) *
+          array32 (word.add p_addr (word.of_Z 104)) bufr)%type *
+         (p_addr + lit 36) |-> lit 4294967295 *
+         (word.add p_addr (lit 32) |-> lit 4294967295 *
+          (word.add p_addr (lit 28) |-> lit 4294967295 *
+           (word.add p_addr (lit 24) |-> lit 4294967295 *
+            (word.add p_addr (lit 20) |-> lit 4294967295 *
+             (word.add p_addr (lit 16) |-> lit 316 *
+              (word.add p_addr (lit 12) |-> lit 164 *
+               (word.add p_addr (lit 8) |-> lit 64 *
+                (word.add p_addr (lit 4) |-> lit 64 *
+                 (p_addr |-> lit 5 * R)))))))))%type) M
+       )) _ _ _ _ _ _ _);
+      cbn [reconstruct map.putmany_of_list HList.tuple.to_list
+           HList.hlist.foralls HList.tuple.foralls
+           HList.hlist.existss HList.tuple.existss
+           HList.hlist.apply  HList.tuple.apply
+           HList.hlist
+
+           List.repeat Datatypes.length
+           HList.polymorphic_list.repeat HList.polymorphic_list.length
+           PrimitivePair.pair._1 PrimitivePair.pair._2] in *.
+
+     (*{  Set Printing All. Check array32.
+        Check (fun V T M I BUFFER =>
+       V = word.unsigned I /\ word.unsigned I <> 0 /\ BUFFER = p_addr /\ exists i, (i < 16)%nat /\ I = word.of_Z (Z.of_nat (64 - 4*i)%nat) /\ (array32  BUFFER nil) M
+       ).*)
+     { repeat straightline. }
+     { eapply (Z.lt_wf 0). }
+     { repeat straightline.
+       shelve. }
+     { repeat (split; trivial; []).
+       subst i; split; try split; auto.
+       - rewrite word.unsigned_of_Z.
+         unfold word.wrap.
+         change width with 32.
+         admit.
+       - exists 0%nat; split; try blia.
+         split; try f_equal.
+         cbn [List.repeat Array.array].
+         replace (word.add (word.add p_addr (word.of_Z 40)) (word.of_Z (Z.of_nat (4 * 0)))) with (word.add p_addr (word.of_Z 40)) by admit.
+         rewrite List.skipn_O.
+         ecancel_assumption. }
+     repeat straightline.
+     subst i a8 x.
+     replace (word.sub (p_addr + word.of_Z 104)
+       (word.sub (word.of_Z (Z.of_nat (64 - 4 * x1))) (word.of_Z 4))) with (word.add (word.add p_addr (word.of_Z 40)) (word.of_Z (Z.of_nat (4 * x1)))) by admit.
+
+     assert (List.length (List.skipn x1 bufl) <> 0%nat).
+     { rewrite List.skipn_length.
+       rewrite H11.
+       blia. }
+     destruct (List.skipn x1 bufl) eqn:H20; try contradiction.
+     cbn[Array.array] in H19.
+     repeat straightline.
+     { eexists; auto.
+       subst v9 x.
+       split.
+       - split; auto.
+         split; try split; auto; try blia.
+         exists (x1 + 1)%nat.
+         split. 1: admit.
+         split. 1: admit.
+         use_sep_assumption.
+         cancel.
+         cancel_seps_at_indices 2%nat 1%nat.
+         { admit. }
+         match goal with
+         | |- context [List.repeat ?x (?n + 1)] =>
+           replace (List.repeat x (n + 1)) with (List.repeat x n ++ [x])
+         end.
+         { 
+           match goal with
+           | |- context [ @array ?w ?word ?v ?m ?T ?PT ?SZ ?start (?xs ++ ?ys) ] =>
+             pose proof iff1ToEq (@array_append w word _ v m _ T PT SZ xs ys start)
+           end.
+           Set Printing All.
+           pose proof iff1ToEq (array_append scalar32 (word.of_Z 4) (List.repeat (lit (Ox "42")) x1) [lit (Ox "42")] (word.add p_addr (lit 40))).
+           Unset Printing All.
+           rewrite H21.
+           Set Printing All.
+           
+           cbn[seps].
+           rewrite H16.
+           Set Printing All.
+           Check (@Datatypes.app
+                (@word.rep (Zpos (xO (xO (xO (xO (xO xH))))))
+                   (@Semantics.word (@semantics_parameters p)))
+                (@List.repeat
+                   (@word.rep (@width (@semantics_parameters p))
+                      (@Semantics.word (@semantics_parameters p)))
+                   (@word.of_Z (@width (@semantics_parameters p))
+                      (@Semantics.word (@semantics_parameters p))
+                      (Ox
+                         (String
+                            (Ascii.Ascii false false true false true true false
+                               false)
+                            (String
+                               (Ascii.Ascii false true false false true true false
+                                  false) EmptyString)))) x1)
+                (@cons
+                   (@word.rep (@width (@semantics_parameters p))
+                      (@Semantics.word (@semantics_parameters p)))
+                   (@word.of_Z (@width (@semantics_parameters p))
+                      (@Semantics.word (@semantics_parameters p))
+                      (Ox
+                         (String
+                            (Ascii.Ascii false false true false true true false
+                               false)
+                            (String
+                               (Ascii.Ascii false true false false true true false
+                                  false) EmptyString))))
+                   (@nil
+                      (@word.rep (@width (@semantics_parameters p))
+                         (@Semantics.word (@semantics_parameters p)))))).
+           rewrite H16.
+           rewr get_array_rewr_eq in *.
+           idtac.
+           Ltac get_array_rewr_eq t :=
+             lazymatch t with
+             | context [ array ?PT ?SZ ?start (?xs ++ ?ys) ] =>
+               constr:(iff1ToEq (array_append PT SZ xs ys start))
+             | context [ array ?PT ?SZ ?start (?x :: ?xs) ] =>
+               constr:(iff1ToEq (array_cons PT SZ x xs start))
+             | context [ array ?PT ?SZ ?start nil ] =>
+               constr:(iff1ToEq (array_nil PT SZ start))
+             end.
+
+           rewrite List.repeat_length.
+           cbn[seps].
+           cancel.
+           
+           pose proof (array_append scalar32 (word.of_Z 4) (List.repeat (word.of_Z (Ox "42")) x1) [word.of_Z (Ox "42")] (p_addr + word.of_Z 40)).
+           SeparationLogic.seprewrite H16.
+
+         
+         replace (List.repeat (word.of_Z (Ox "42")) (x1 + 1)) with (List.repeat (word.of_Z (Ox "42")) x1 ++ [word.of_Z (Ox "42")]).
+         
+         canonicalize_word_width_and_instance.
+         
+         replace (List.repeat (A := Semantics.word) (word.of_Z (Ox "42")) (x1 + 1)) with (List.repeat (word.of_Z (Ox "42")) x1 ++ [word.of_Z (Ox "42")]).
+     
+     ring_simplify (word.sub (p_addr + word.of_Z 104)
+       (word.sub (word.of_Z (Z.of_nat (64 - 4 * x1))) (word.of_Z 4))).
+     straightline.
+
+
+     
+     { repeat (split; trivial; []).
+       subst i; split; try split; auto.
+       - rewrite word.unsigned_of_Z.
+         unfold word.wrap.
+         change width with 32.
+         admit.
+       - exists 0%nat; split. 1: admit.
+         cbn [List.repeat Array.array].
+         replace (word.add (word.add p_addr (word.of_Z 40)) (word.of_Z 0)) with (word.add p_addr (word.of_Z 40)) by ring.
+         rewrite List.skipn_O.
+         ecancel_assumption.
+     }
+     
+     repeat straightline.
+     assert (List.length (List.skipn x1 bufl) <> 0%nat).
+     { rewrite List.skipn_length.
+       rewrite <- H17 in H14.
+       blia. }
+     destruct (List.skipn x1 bufl) eqn:H20; try contradiction.
+     cbn[Array.array] in H18.
+     repeat straightline.
+     { eexists; split.
+       - split; auto.
+         subst i.
+         split. 1: admit.
+         split; auto.
+         exists (x1 + 1)%nat.
+         split. 1: admit.
+         replace ((x1+1)%nat) with (S x1) by blia.
+         rewrite <- List.tl_skipn, H20.
+         cbv [List.tl].
+         assert (List.repeat (word.of_Z (word := parameters.word) (Ox "42")) (S x1) = List.repeat (word.of_Z (Ox "42")) x1 ++ [word.of_Z (Ox "42")]) by admit.
+         rewrite H21.
+         admit.
+       - subst i v9.
+         
+     }
+         
+         replace (List.repeat (word.of_Z (Ox "42")) (S x1)) with ((List.repeat (word.of_Z (Ox "42")) x1) ++ [word.of_Z (Ox "42")]).
+         Search List.repeat_cons.
+
+         ecancel_assumption.
+         List.repeat Array.array].
+         
+         ecancel_assumption.
+         Search List.skipn.
+         
+         ecancel H16.
+
+         
+     Search List.skipn List.length.
+     subst a8.
+     straightline.
+     eapply WeakestPreconditionProperties.interact_nomem; repeat straightline.
+     
+     
+
+     refine ((atleastonce ["i"; "buffer"] (fun v T M I BUFFER =>
+       v = word.unsigned I /\ word.unsigned I <> 0 /\ M = m 
+       
+      )) _ _ _ _ _ _ _);
+      cbn [reconstruct map.putmany_of_list HList.tuple.to_list
+           HList.hlist.foralls HList.tuple.foralls
+           HList.hlist.existss HList.tuple.existss
+           HList.hlist.apply  HList.tuple.apply
+           HList.hlist
+           List.repeat Datatypes.length
+           HList.polymorphic_list.repeat HList.polymorphic_list.length
+           PrimitivePair.pair._1 PrimitivePair.pair._2] in *.
+
+     { repeat straightline. }
+     { eapply (Z.lt_wf 0). }
+     { eexists; split; repeat straightline.
+       subst i. rewrite word.unsigned_of_Z in H; inversion H. }
+     { repeat (split; trivial; []).
+       subst i. rewrite word.unsigned_of_Z.
+       split.
+       { discriminate. }
+       split; trivial.
+       eexists; split.
+       { rewrite app_nil_l; trivial. }
+       eexists; split.
+       { constructor. }
+       split.
+       { constructor. }
+       exact eq_refl. }
+     repeat straightline.
+     
+     refine ((atleastonce ["b"; "busy"; "i"] (fun v T M B BUSY I =>
+       b = B /\ v = word.unsigned I /\ word.unsigned I <> 0 /\ M = m /\
+       exists tl, T = tl++t /\
+       exists th, mmio_trace_abstraction_relation th tl /\
+       lightbulb_spec.spi_write_full _ ^* th /\
+       Z.of_nat (length th) + word.unsigned I = patience
+       )) _ _ _ _ _ _ _);
+      cbn [reconstruct map.putmany_of_list HList.tuple.to_list
+           HList.hlist.foralls HList.tuple.foralls
+           HList.hlist.existss HList.tuple.existss
+           HList.hlist.apply  HList.tuple.apply
+           HList.hlist
+           List.repeat Datatypes.length
+           HList.polymorphic_list.repeat HList.polymorphic_list.length
+           PrimitivePair.pair._1 PrimitivePair.pair._2] in *.
+     
+     refine ((TailRecursion.atleastonce ["i"; "buffer"] (fun v T M I BUFFER =>
+       v = word.unsigned I /\ word.unsigned I <> 0 /\ M = m
+       )) _ _ _ _ _ _ _);
+      cbn [reconstruct map.putmany_of_list HList.tuple.to_list
+           HList.hlist.foralls HList.tuple.foralls
+           HList.hlist.existss HList.tuple.existss
+           HList.hlist.apply  HList.tuple.apply
+           HList.hlist
+
+           List.repeat Datatypes.length
+           HList.polymorphic_list.repeat HList.polymorphic_list.length
+           PrimitivePair.pair._1 PrimitivePair.pair._2] in *.
+     { repeat straightline. }
+     { eapply (Z.lt_wf 0). }
+     {   repeat straightline. subst i.
+         assert (br = word.of_Z 1). { subst br. reflexivity.
+         change (word.unsigned (word.of_Z 1) = 0) in H11. 
+     { move c6 at bottom. eexists; split; repeat straightline.
+       subst i. rewrite word.unsigned_of_Z in H; inversion H. }
+    
+     
+     hnf in c.
+     
+     let c := eval hnf in c in
+         lazymatch c with
+         | cmd.while _ _ => fail
+         | cmd.cond _ _ _ => fail
+         | cmd.interact _ _ _ => fail
+         | _ => WeakestPrecondition.unfold1_cmd_goal; cbv beta match delta [cmd_body]
+         end.
+
+     current_trace_mem_locals.
+
+     
+     split; [auto|].
+     split; [auto|].
+     clear H9 H8 H7 H6 H5 H4 H3 H2 H1 H.
+     subst v v0 v1 v2 v3 v4 v5 v6 v7 v8.
+     repeat (rewrite word.unsigned_of_Z in H10).
+     unfold word.wrap in H10.
+     repeat (rewrite Zmod_small in H10 ;
+             [|change width with 32; try apply stringHexBound; blia]).
+     subst a a0 a1 a2 a3 a4 a5 a6 a7.
+     cbv [message_val message_ok size_field offsets_field tags_field srep_val
+                      List.fold_left snd fst List.map contents_offset tl
+                      List.length tags_offset Nat.mul Nat.add stringToWord].
+     cbv[Array.array].
+     repeat (rewrite word_add_simplify).
+     simpl.
+     use_sep_assumption.
+     simpl.
+     cancel.
+     simpl.
+     cancel.
+     cancel_seps_at_indices 9%nat 0%nat.
+     Set Printing All.
+     ecancel.
+     Search (Lift1Prop.iff1 _ _ -> _).
+     simpl.
+     cancel.
+     word_simplify.
+     ecancel.
+     cancel_seps_at_indices 9%nat 0%nat.
+     simpl. Set Printing All. 
+     unfold message_ok.
+     subst a5.
+     straightline_cleanup.
+     
+     match goal with | |- @WeakestPrecondition.store ?p access_size.four _ _ _ _ =>
+      eapply (@Scalars.store_four_of_sep (@Semantics.width p) (@Semantics.word p) _ _ _ _ _) ; [solve[ecancel_assumption]|] end.
+     straightline.
+     replace buf with ([word.of_Z 4]++[word.of_Z 3]) in H. 2: admit.
+     rewrite (iff1ToEq (array_append _ _ _ _ _)) in H.
+     straightline.
+
+     seprewrite_in (array_append scalar32 (word.of_Z 4) [word.of_Z 4] [word.of_Z 3]) H. 
+     rewrite (array_append) in H.
+     (* Start with header *)
+     erewrite (array_index_nat_inbounds) in H.
+     do 10 (destruct buf; [inversion H0|]).
+     rewrite (array_append ) in H.
+     cbn[Array.array] in H.
+     word_simplify.
+     repeat straightline.
+     split; [auto|].
+     split; [auto|].
+     unfold v, v0, v1, v2, v3, v4, v5, v6, v7, v8 in *.
+     repeat (rewrite word.unsigned_of_Z in H10).
+     unfold word.wrap in H10.
+     repeat (rewrite Zmod_small in H10 ;
+             [|change width with 32; try apply stringHexBound; blia]).
+     unfold a, a0, a1, a2, a3, a4, a5, a6, a7 in H10.
+     simpl.
+     unfold size_ok, offsets_ok, tags_ok, contents_offset, tags_offset.
+     simpl.
+     word_simplify.
+   Admitted.
+                                 
    
    Lemma createTimestampMessage_ok : program_logic_goal_for_function! createTimestampMessage.
    Proof.
@@ -140,6 +959,7 @@ Section WithParameters.
      simpl.
      unfold size_ok, offsets_ok, tags_ok, contents_offset, tags_offset.
      simpl.
+     word_simplify.
    Admitted.
    
 End WithParameters.
